library/init/meta/default.lean
@@ -11,5 +11,5 @@ import init.meta.injection_tactic init.meta.relation_tactics init.meta.fun_info
 import init.meta.congr_lemma init.meta.match_tactic init.meta.ac_tactics
 import init.meta.backward init.meta.rewrite_tactic init.meta.unfold_tactic
 import init.meta.mk_dec_eq_instance init.meta.mk_inhabited_instance
-import init.meta.simp_tactic init.meta.defeq_simp_tactic init.meta.set_get_option_tactics
+import init.meta.simp_tactic init.meta.set_get_option_tactics
 import init.meta.interactive init.meta.converter
